State soundness and type_soundness separately.

F_mu/fundamental.v
@@ -3,10 +3,14 @@ From iris.proofmode Require Import tactics.
 From iris_logrel.F_mu Require Import rules.
 From iris.algebra Require Export upred_big_op.
 
-Section typed_interp.
+Definition log_typed {Σ} (Γ : list type) (e : expr) (τ : type) := ∀ Δ vs,
+  @env_PersistentP Σ Δ →
+  ⟦ Γ ⟧* Δ vs ⊢ ⟦ τ ⟧ₑ Δ e.[env_subst vs].
+Notation "Γ ⊨ e : τ" := (log_typed Γ e τ) (at level 74, e, τ at next level).
+
+Section fundamental.
   Context {Σ : iFunctor}.
   Notation D := (valC -n> iProp lang Σ).
-  Implicit Types Δ : listC D.
 
   Local Tactic Notation "smart_wp_bind" uconstr(ctx) ident(v) constr(Hv) uconstr(Hp) :=
     iApply (@wp_bind _ _ _ [ctx]);
@@ -16,74 +20,72 @@ Section typed_interp.
 
   Local Ltac value_case := iApply wp_value; cbn; rewrite ?to_of_val; trivial.
 
-  Theorem fundamental Δ Γ vs e τ (HΔ : env_PersistentP Δ) :
-    Γ ⊢ₜ e : τ → ⟦ Γ ⟧* Δ vs ⊢ ⟦ τ ⟧ₑ Δ e.[env_subst vs].
+  Theorem fundamental Γ e τ : Γ ⊢ₜ e : τ → log_typed (Σ:=Σ) Γ e τ.
   Proof.
-    intros Htyped. revert Δ vs HΔ.
-    induction Htyped; iIntros {Δ vs HΔ} "#HΓ"; cbn.
+    induction 1; iIntros {Δ vs HΔ} "#HΓ"; cbn.
     - (* var *)
       iDestruct (interp_env_Some_l with "HΓ") as {v} "[% ?]"; first done.
       rewrite /env_subst. simplify_option_eq. by value_case.
     - (* unit *) value_case.
     - (* pair *)
-      smart_wp_bind (PairLCtx e2.[env_subst vs]) v "# Hv" IHHtyped1.
-      smart_wp_bind (PairRCtx v) v' "# Hv'" IHHtyped2.
+      smart_wp_bind (PairLCtx e2.[env_subst vs]) v "# Hv" IHtyped1.
+      smart_wp_bind (PairRCtx v) v' "# Hv'" IHtyped2.
       value_case; eauto 10.
     - (* fst *)
-      smart_wp_bind (FstCtx) v "# Hv" IHHtyped; cbn.
+      smart_wp_bind (FstCtx) v "# Hv" IHtyped; cbn.
       iDestruct "Hv" as {w1 w2} "#[% [H2 H3]]"; subst.
       iApply wp_fst; eauto using to_of_val.
     - (* snd *)
-      smart_wp_bind (SndCtx) v "# Hv" IHHtyped; cbn.
+      smart_wp_bind (SndCtx) v "# Hv" IHtyped; cbn.
       iDestruct "Hv" as {w1 w2} "#[% [H2 H3]]"; subst.
       iApply wp_snd; eauto using to_of_val.
     - (* injl *)
-      smart_wp_bind (InjLCtx) v "# Hv" IHHtyped; cbn.
+      smart_wp_bind (InjLCtx) v "# Hv" IHtyped; cbn.
       value_case; eauto.
     - (* injr *)
-      smart_wp_bind (InjRCtx) v "# Hv" IHHtyped; cbn.
+      smart_wp_bind (InjRCtx) v "# Hv" IHtyped; cbn.
       value_case; eauto.
     - (* case *)
-      smart_wp_bind (CaseCtx _ _) v "#Hv" IHHtyped1; cbn.
+      smart_wp_bind (CaseCtx _ _) v "#Hv" IHtyped1; cbn.
       iDestruct (interp_env_length with "HΓ") as %?.
       iDestruct "Hv" as "[Hv|Hv]"; iDestruct "Hv" as {w} "[% Hw]"; simplify_eq/=.
       + iApply wp_case_inl; auto 1 using to_of_val; asimpl. iNext.
         erewrite typed_subst_head_simpl by naive_solver.
-        iApply (IHHtyped2 Δ (w :: vs)). iApply interp_env_cons; auto.
+        iApply (IHtyped2 Δ (w :: vs)). iApply interp_env_cons; auto.
       + iApply wp_case_inr; auto 1 using to_of_val; asimpl. iNext.
         erewrite typed_subst_head_simpl by naive_solver.
-        iApply (IHHtyped3 Δ (w :: vs)). iApply interp_env_cons; auto.
+        iApply (IHtyped3 Δ (w :: vs)). iApply interp_env_cons; auto.
     - (* lam *)
       value_case; iAlways; iIntros {w} "#Hw".
       iDestruct (interp_env_length with "HΓ") as %?.
       iApply wp_lam; auto 1 using to_of_val. iNext.
       asimpl. erewrite typed_subst_head_simpl by naive_solver.
-      iApply (IHHtyped Δ (w :: vs)). iApply interp_env_cons; auto.
+      iApply (IHtyped Δ (w :: vs)). iApply interp_env_cons; auto.
     - (* app *)
-      smart_wp_bind (AppLCtx (e2.[env_subst vs])) v "#Hv" IHHtyped1.
-      smart_wp_bind (AppRCtx v) w "#Hw" IHHtyped2.
+      smart_wp_bind (AppLCtx (e2.[env_subst vs])) v "#Hv" IHtyped1.
+      smart_wp_bind (AppRCtx v) w "#Hw" IHtyped2.
       iApply wp_mono; [|iApply "Hv"]; auto.
     - (* TLam *)
       value_case.
       iAlways; iIntros { τi } "%". iApply wp_TLam; iNext.
-      iApply IHHtyped. by iApply interp_env_ren.
+      iApply IHtyped. by iApply interp_env_ren.
     - (* TApp *)
-      smart_wp_bind TAppCtx v "#Hv" IHHtyped; cbn.
+      smart_wp_bind TAppCtx v "#Hv" IHtyped; cbn.
       iApply wp_wand_r; iSplitL; [iApply ("Hv" $! (⟦ τ' ⟧ Δ)); iPureIntro; apply _|].
       iIntros {w} "?". by rewrite interp_subst.
     - (* Fold *)
       iApply (@wp_bind _ _ _ [FoldCtx]);
-        iApply wp_wand_l; iSplitL; [|iApply (IHHtyped Δ vs); auto].
+        iApply wp_wand_l; iSplitL; [|iApply (IHtyped Δ vs); auto].
       iIntros {v} "#Hv". value_case.
       rewrite /= -interp_subst fixpoint_unfold /=.
       iAlways; eauto.
     - (* Unfold *)
       iApply (@wp_bind _ _ _ [UnfoldCtx]);
-        iApply wp_wand_l; iSplitL; [|iApply IHHtyped; trivial].
+        iApply wp_wand_l; iSplitL; [|iApply IHtyped; trivial].
       iIntros {v} "#Hv". rewrite /= fixpoint_unfold.
       change (fixpoint _) with (⟦ TRec τ ⟧ Δ); simpl.
       iDestruct "Hv" as {w} "#[% Hw]"; subst.
       iApply wp_Fold; cbn; auto using to_of_val.
       by rewrite -interp_subst.
   Qed.
-End typed_interp.
+End fundamental.
