F_mu_ref_par/fundamental_unary.v
@@ -3,10 +3,14 @@ From iris_logrel.F_mu_ref_par Require Import rules.
 From iris.algebra Require Export upred_big_op.
 From iris.proofmode Require Import tactics pviewshifts invariants.
 
+Definition log_typed `{heapIG Σ} (Γ : list type) (e : expr) (τ : type) := ∀ Δ vs,
+  env_PersistentP Δ →
+  heapI_ctx ∧ ⟦ Γ ⟧* Δ vs ⊢ ⟦ τ ⟧ₑ Δ e.[env_subst vs].
+Notation "Γ ⊨ e : τ" := (log_typed Γ e τ) (at level 74, e, τ at next level).
+
 Section typed_interp.
   Context `{heapIG Σ}.
   Notation D := (valC -n> iPropG lang Σ).
-  Implicit Types Δ : listC D.
 
   Local Tactic Notation "smart_wp_bind" uconstr(ctx) ident(v) constr(Hv) uconstr(Hp) :=
     iApply (@wp_bind _ _ _ [ctx]);
@@ -15,12 +19,9 @@ Section typed_interp.
 
   Local Ltac value_case := iApply wp_value; [cbn; rewrite ?to_of_val; trivial|].
 
-  Theorem fundamental Δ Γ vs e τ (HΔ : env_PersistentP Δ) :
-    Γ ⊢ₜ e : τ →
-    heapI_ctx ∧ ⟦ Γ ⟧* Δ vs ⊢ ⟦ τ ⟧ₑ Δ e.[env_subst vs].
+  Theorem fundamental Γ e τ : Γ ⊢ₜ e : τ → Γ ⊨ e : τ.
   Proof.
-    intros Htyped; revert Δ vs HΔ.
-    induction Htyped; iIntros {Δ vs HΔ} "#[Hheap HΓ] /=".
+    induction 1; iIntros {Δ vs HΔ} "#[Hheap HΓ] /=".
     - (* var *)
       iDestruct (interp_env_Some_l with "HΓ") as {v} "[% ?]"; first done.
       rewrite /env_subst. simplify_option_eq. by value_case.
@@ -28,74 +29,74 @@ Section typed_interp.
     - (* nat *) value_case; simpl; eauto.
     - (* bool *) value_case; simpl; eauto.
     - (* nat bin op *)
-      smart_wp_bind (BinOpLCtx _ e2.[env_subst vs]) v "#Hv" IHHtyped1.
-      smart_wp_bind (BinOpRCtx _ v) v' "# Hv'" IHHtyped2.
+      smart_wp_bind (BinOpLCtx _ e2.[env_subst vs]) v "#Hv" IHtyped1.
+      smart_wp_bind (BinOpRCtx _ v) v' "# Hv'" IHtyped2.
       iDestruct "Hv" as {n} "%"; iDestruct "Hv'" as {n'} "%"; simplify_eq/=.
       iApply wp_nat_binop. iNext; iPvsIntro. iClear "Hheap HΓ".
       destruct op; simpl; try destruct eq_nat_dec;
         try destruct le_dec; try destruct lt_dec; eauto 10.
     - (* pair *)
-      smart_wp_bind (PairLCtx e2.[env_subst vs]) v "#Hv" IHHtyped1.
-      smart_wp_bind (PairRCtx v) v' "# Hv'" IHHtyped2.
+      smart_wp_bind (PairLCtx e2.[env_subst vs]) v "#Hv" IHtyped1.
+      smart_wp_bind (PairRCtx v) v' "# Hv'" IHtyped2.
       value_case; eauto.
     - (* fst *)
-      smart_wp_bind (FstCtx) v "# Hv" IHHtyped; cbn.
+      smart_wp_bind (FstCtx) v "# Hv" IHtyped; cbn.
       iDestruct "Hv" as {w1 w2} "#[% [H2 H3]]"; subst.
       iApply wp_fst; eauto using to_of_val.
     - (* snd *)
-      smart_wp_bind (SndCtx) v "# Hv" IHHtyped; cbn.
+      smart_wp_bind (SndCtx) v "# Hv" IHtyped; cbn.
       iDestruct "Hv" as {w1 w2} "#[% [H2 H3]]"; subst.
       iApply wp_snd; eauto using to_of_val.
     - (* injl *)
-      smart_wp_bind (InjLCtx) v "# Hv" IHHtyped; cbn.
+      smart_wp_bind (InjLCtx) v "# Hv" IHtyped; cbn.
       value_case; eauto.
     - (* injr *)
-      smart_wp_bind (InjRCtx) v "# Hv" IHHtyped; cbn.
+      smart_wp_bind (InjRCtx) v "# Hv" IHtyped; cbn.
       value_case; eauto.
     - (* case *)
-      smart_wp_bind (CaseCtx _ _) v "#Hv" IHHtyped1; cbn.
+      smart_wp_bind (CaseCtx _ _) v "#Hv" IHtyped1; cbn.
       iDestruct (interp_env_length with "HΓ") as %?.
       iDestruct "Hv" as "[Hv|Hv]"; iDestruct "Hv" as {w} "[% Hw]"; simplify_eq/=.
       + iApply wp_case_inl; auto 1 using to_of_val; asimpl. iNext.
         erewrite typed_subst_head_simpl by naive_solver.
-        iApply (IHHtyped2 Δ (w :: vs)). iSplit; [|iApply interp_env_cons]; auto.
+        iApply (IHtyped2 Δ (w :: vs)). iSplit; [|iApply interp_env_cons]; auto.
       + iApply wp_case_inr; auto 1 using to_of_val; asimpl. iNext.
         erewrite typed_subst_head_simpl by naive_solver.
-        iApply (IHHtyped3 Δ (w :: vs)). iSplit; [|iApply interp_env_cons]; auto.
+        iApply (IHtyped3 Δ (w :: vs)). iSplit; [|iApply interp_env_cons]; auto.
     - (* If *)
-      smart_wp_bind (IfCtx _ _) v "#Hv" IHHtyped1; cbn.
+      smart_wp_bind (IfCtx _ _) v "#Hv" IHtyped1; cbn.
       iDestruct "Hv" as { [] } "%"; subst; simpl;
         [iApply wp_if_true| iApply wp_if_false]; iNext;
-      [iApply IHHtyped2| iApply IHHtyped3]; auto.
+      [iApply IHtyped2| iApply IHtyped3]; auto.
     - (* Rec *)
       value_case; iAlways. simpl. iLöb as "IH"; iIntros {w} "#Hw".
       iDestruct (interp_env_length with "HΓ") as %?.
       iApply wp_rec; auto 1 using to_of_val. iNext.
       asimpl. change (Rec _) with (# (RecV e.[upn 2 (env_subst vs)])).
       erewrite typed_subst_head_simpl_2 by naive_solver.
-      iApply (IHHtyped Δ (_ :: w :: vs)). iSplit; [done|].
+      iApply (IHtyped Δ (_ :: w :: vs)). iSplit; [done|].
       iApply interp_env_cons; iSplit; [|iApply interp_env_cons]; auto.
     - (* app *)
-      smart_wp_bind (AppLCtx (e2.[env_subst vs])) v "#Hv" IHHtyped1.
-      smart_wp_bind (AppRCtx v) w "#Hw" IHHtyped2.
+      smart_wp_bind (AppLCtx (e2.[env_subst vs])) v "#Hv" IHtyped1.
+      smart_wp_bind (AppRCtx v) w "#Hw" IHtyped2.
       iApply wp_mono; [|iApply "Hv"]; auto.
     - (* TLam *)
       value_case.
       iAlways; iIntros { τi } "%". iApply wp_tlam; iNext.
-      iApply IHHtyped. iFrame "Hheap". by iApply interp_env_ren.
+      iApply IHtyped. iFrame "Hheap". by iApply interp_env_ren.
     - (* TApp *)
-      smart_wp_bind TAppCtx v "#Hv" IHHtyped; cbn.
+      smart_wp_bind TAppCtx v "#Hv" IHtyped; cbn.
       iApply wp_wand_r; iSplitL; [iApply ("Hv" $! (⟦ τ' ⟧ Δ)); iPureIntro; apply _|]; cbn.
       iIntros {w} "?". by iApply interp_subst.
     - (* Fold *)
       iApply (@wp_bind _ _ _ [FoldCtx]);
-        iApply wp_wand_l; iSplitL; [|iApply (IHHtyped Δ vs); auto].
+        iApply wp_wand_l; iSplitL; [|iApply (IHtyped Δ vs); auto].
       iIntros {v} "#Hv". value_case.
       rewrite /= -interp_subst fixpoint_unfold /=.
       iAlways; eauto.
     - (* Unfold *)
       iApply (@wp_bind _ _ _ [UnfoldCtx]);
-        iApply wp_wand_l; iSplitL; [|iApply IHHtyped; auto].
+        iApply wp_wand_l; iSplitL; [|iApply IHtyped; auto].
       iIntros {v} "#Hv". rewrite /= fixpoint_unfold.
       change (fixpoint _) with (⟦ TRec τ ⟧ Δ); simpl.
       iDestruct "Hv" as {w} "#[% Hw]"; subst.
@@ -103,9 +104,9 @@ Section typed_interp.
       iNext; iPvsIntro. by iApply interp_subst.
     - (* Fork *)
       iApply wp_fork. iNext; iSplitL; trivial.
-      iApply wp_wand_l. iSplitL; [|iApply IHHtyped; auto]; auto.
+      iApply wp_wand_l. iSplitL; [|iApply IHtyped; auto]; auto.
     - (* Alloc *)
-      smart_wp_bind AllocCtx v "#Hv" IHHtyped; cbn. iClear "HΓ".
+      smart_wp_bind AllocCtx v "#Hv" IHtyped; cbn. iClear "HΓ".
       iApply wp_atomic; cbn; trivial; [rewrite to_of_val; auto|].
       iPvsIntro.
       iApply wp_alloc; auto 1 using to_of_val.
@@ -114,7 +115,7 @@ Section typed_interp.
       iPvs (inv_alloc _ with "[Hl]") as "HN";
         [| | iPvsIntro; iExists _; iSplit; trivial]; eauto.
     - (* Load *)
-      smart_wp_bind LoadCtx v "#Hv" IHHtyped; cbn. iClear "HΓ".
+      smart_wp_bind LoadCtx v "#Hv" IHtyped; cbn. iClear "HΓ".
       iDestruct "Hv" as {l} "[% #Hv]"; subst.
       iApply wp_atomic; cbn; eauto using to_of_val.
       iPvsIntro.
@@ -122,8 +123,8 @@ Section typed_interp.
       iApply (wp_load _ _ 1); [|iFrame "Hheap"]; trivial. solve_ndisj.
       iIntros "{$Hw1} > Hw1". iPvsIntro; iSplitL; eauto.
     - (* Store *)
-      smart_wp_bind (StoreLCtx _) v "#Hv" IHHtyped1; cbn.
-      smart_wp_bind (StoreRCtx _) w "#Hw" IHHtyped2; cbn. iClear "HΓ".
+      smart_wp_bind (StoreLCtx _) v "#Hv" IHtyped1; cbn.
+      smart_wp_bind (StoreRCtx _) w "#Hw" IHtyped2; cbn. iClear "HΓ".
       iDestruct "Hv" as {l} "[% #Hv]"; subst.
       iApply wp_atomic; cbn; [trivial| rewrite ?to_of_val; auto |].
       iPvsIntro.
@@ -132,9 +133,9 @@ Section typed_interp.
       iApply wp_store; auto using to_of_val. solve_ndisj.
       iIntros "{$Hheap $Hz1} > Hz1". iPvsIntro. iSplitL; eauto 10.
     - (* CAS *)
-      smart_wp_bind (CasLCtx _ _) v1 "#Hv1" IHHtyped1; cbn.
-      smart_wp_bind (CasMCtx _ _) v2 "#Hv2" IHHtyped2; cbn.
-      smart_wp_bind (CasRCtx _ _) v3 "#Hv3" IHHtyped3; cbn. iClear "HΓ".
+      smart_wp_bind (CasLCtx _ _) v1 "#Hv1" IHtyped1; cbn.
+      smart_wp_bind (CasMCtx _ _) v2 "#Hv2" IHtyped2; cbn.
+      smart_wp_bind (CasRCtx _ _) v3 "#Hv3" IHtyped3; cbn. iClear "HΓ".
       iDestruct "Hv1" as {l} "[% Hinv]"; subst.
       iApply wp_atomic; cbn; eauto 10 using to_of_val.
       iPvsIntro.
