F_mu/soundness.v
@@ -2,22 +2,22 @@ From iris_logrel.F_mu Require Export fundamental.
 From iris.proofmode Require Import tactics.
 From iris.program_logic Require Import adequacy.
 
-Section soundness.
-  Let Σ := #[].
+Theorem soundness Σ e τ e' thp σ σ' :
+  log_typed (Σ:=Σ) [] e τ →
+  rtc step ([e], σ) (e' :: thp, σ') →
+  is_Some (to_val e') ∨ reducible e' σ'.
+Proof.
+  intros Hlog ?. eapply (wp_adequacy_reducible ⊤ (λ _, True%I));
+    eauto using ucmra_unit_valid; last by constructor.
+  iIntros "_". rewrite -(empty_env_subst e).
+  iApply wp_wand_l; iSplitR; [|iApply Hlog]; eauto. by iApply interp_env_nil.
+Qed.
 
-  Lemma wp_soundness e τ :
-    [] ⊢ₜ e : τ → True ⊢ WP e {{ @interp (globalF Σ) τ [] }}.
-  Proof.
-    iIntros {H} "". rewrite -(empty_env_subst e).
-    iApply (@fundamental _ _ _ []); eauto. by iApply interp_env_nil.
-  Qed.
-
-  Theorem soundness e τ e' thp :
-    [] ⊢ₜ e : τ → rtc step ([e], ()) (e' :: thp, ()) →
-    is_Some (to_val e') ∨ reducible e' ().
-  Proof.
-    intros ??. eapply wp_adequacy_reducible; eauto using ucmra_unit_valid.
-    - iIntros "H". by iApply wp_soundness.
-    - constructor.
-  Qed.
-End soundness.
+Lemma type_soundness e τ e' thp σ σ' :
+  [] ⊢ₜ e : τ →
+  rtc step ([e], σ) (e' :: thp, σ') →
+  is_Some (to_val e') ∨ reducible e' σ'.
+Proof.
+  set (Σ := #[]).
+  intros Htyped. eapply (@soundness (globalF Σ)), fundamental, Htyped.
+Qed.
