F_mu_ref_par/soundness_unary.v
@@ -1,28 +1,26 @@
 From iris_logrel.F_mu_ref_par Require Export fundamental_unary.
 From iris.proofmode Require Import tactics pviewshifts.
-From iris.program_logic Require Import ownership adequacy.
+From iris.program_logic Require Import ownership adequacy auth.
 
-Section soundness.
-  Let Σ := #[ auth.authGF heapUR ].
+Theorem soundness `{authG lang Σ heapUR} e τ e' thp σ σ' :
+  (∀ `{heapIG Σ}, [] ⊨ e : τ) →
+  rtc step ([e], σ) (e' :: thp, σ') →
+  is_Some (to_val e') ∨ reducible e' σ'.
+Proof.
+  intros Hlog ?. eapply (wp_adequacy_reducible ⊤ (λ _, True%I));
+    eauto using ucmra_unit_valid; last by constructor.
+  iIntros "[Hemp _]".
+  iPvs (heap_alloc with "Hemp") as {h} "[Hheap Hemp]"; first solve_ndisj.
+  rewrite -(empty_env_subst e).
+  iApply wp_wand_l; iSplitR; [|iApply Hlog]; eauto.
+  repeat iSplit; eauto. by iApply interp_env_nil.
+Qed.
 
-  Lemma wp_soundness e τ σ :
-    [] ⊢ₜ e : τ →
-    ownP σ ⊢ WP e {{ v, ∃ H : heapIG Σ, interp τ [] v}}.
-  Proof.
-    iIntros {H1} "Hemp".
-    iPvs (heap_alloc with "Hemp") as {H} "[Hheap Hemp]"; first solve_ndisj.
-    iApply wp_wand_l. iSplitR.
-    { iIntros {v} "HΦ". iExists H. iExact "HΦ". }
-    rewrite -(empty_env_subst e).
-    iApply fundamental; repeat iSplit; eauto. by iApply interp_env_nil.
-  Qed.
-
-  Theorem soundness e τ e' thp σ σ' :
-    [] ⊢ₜ e : τ → rtc step ([e], σ) (e' :: thp, σ') →
-    is_Some (to_val e') ∨ reducible e' σ'.
-  Proof.
-    intros ??. eapply wp_adequacy_reducible; eauto using ucmra_unit_valid.
-    - iIntros "[??]". by iApply wp_soundness.
-    - constructor.
-  Qed.
-End soundness.
+Lemma type_soundness e τ e' thp σ σ' :
+  [] ⊢ₜ e : τ →
+  rtc step ([e], σ) (e' :: thp, σ') →
+  is_Some (to_val e') ∨ reducible e' σ'.
+Proof.
+  set (Σ := #[ auth.authGF heapUR ]).
+  intros Htyped. eapply (@soundness Σ _)=> ?. eapply fundamental, Htyped.
+Qed.
